<?xml version="1.0"?>
<rdf:RDF xmlns="http://ontofox.hegroup.org/zhkxnkhx.owl#"
     xml:base="http://ontofox.hegroup.org/zhkxnkhx.owl"
     xmlns:rdf="http://www.w3.org/1999/02/22-rdf-syntax-ns#"
     xmlns:owl="http://www.w3.org/2002/07/owl#"
     xmlns:xsd="http://www.w3.org/2001/XMLSchema#"
     xmlns:rdfs="http://www.w3.org/2000/01/rdf-schema#"
     xmlns:obo="http://purl.obolibrary.org/obo/">
    <owl:Ontology rdf:about="http://ontofox.hegroup.org/zhkxnkhx.owl"/>
    


    <!-- 
    ///////////////////////////////////////////////////////////////////////////////////////
    //
    // Annotation properties
    //
    ///////////////////////////////////////////////////////////////////////////////////////
     -->

    <owl:AnnotationProperty rdf:about="http://purl.obolibrary.org/obo/IAO_0000118">
        <rdfs:label xml:lang="en">alternative label</rdfs:label>
        <obo:IAO_0000115 xml:lang="en">A label for a class or property that can be used to refer to the class or property instead of the preferred rdfs:label. Alternative labels should be used to indicate community- or context-specific labels, abbreviations, shorthand forms and the like.</obo:IAO_0000115>
    </owl:AnnotationProperty>
    <owl:AnnotationProperty rdf:about="http://purl.obolibrary.org/obo/IAO_0000412">
        <rdfs:label xml:lang="en">imported from</rdfs:label>
    </owl:AnnotationProperty>
    <owl:AnnotationProperty rdf:about="http://purl.obolibrary.org/obo/IAO_0000115">
        <rdfs:label xml:lang="en">definition</rdfs:label>
        <obo:IAO_0000115 xml:lang="en">The official definition, explaining the meaning of a class or property. Shall be Aristotelian, formalized and normalized. Can be augmented with colloquial definitions.</obo:IAO_0000115>
    </owl:AnnotationProperty>
    


    <!-- 
    ///////////////////////////////////////////////////////////////////////////////////////
    //
    // Datatypes
    //
    ///////////////////////////////////////////////////////////////////////////////////////
     -->

    


    <!-- 
    ///////////////////////////////////////////////////////////////////////////////////////
    //
    // Classes
    //
    ///////////////////////////////////////////////////////////////////////////////////////
     -->

    


    <!-- http://purl.obolibrary.org/obo/BFO_0000001 -->

    <owl:Class rdf:about="http://purl.obolibrary.org/obo/BFO_0000001">
        <rdfs:label xml:lang="en">entity</rdfs:label>
        <obo:IAO_0000412 rdf:resource="http://purl.obolibrary.org/obo/obcs.owl"/>
    </owl:Class>
    


    <!-- http://purl.obolibrary.org/obo/BFO_0000002 -->

    <owl:Class rdf:about="http://purl.obolibrary.org/obo/BFO_0000002">
        <rdfs:label xml:lang="en">continuant</rdfs:label>
        <rdfs:subClassOf rdf:resource="http://purl.obolibrary.org/obo/BFO_0000001"/>
        <obo:IAO_0000115 xml:lang="en">An entity that exists in full at any time in which it exists at all, persists through time while maintaining its identity and has no temporal parts.</obo:IAO_0000115>
        <obo:IAO_0000412 rdf:resource="http://purl.obolibrary.org/obo/obcs.owl"/>
    </owl:Class>
    


    <!-- http://purl.obolibrary.org/obo/BFO_0000031 -->

    <owl:Class rdf:about="http://purl.obolibrary.org/obo/BFO_0000031">
        <rdfs:label xml:lang="en">generically dependent continuant</rdfs:label>
        <rdfs:subClassOf rdf:resource="http://purl.obolibrary.org/obo/BFO_0000002"/>
        <obo:IAO_0000115 xml:lang="en">b is a generically dependent continuant = Def. b is a continuant that g-depends_on one or more other entities. (axiom label in BFO2 Reference: [074-001])</obo:IAO_0000115>
        <obo:IAO_0000412 rdf:resource="http://purl.obolibrary.org/obo/obcs.owl"/>
    </owl:Class>
    


    <!-- http://purl.obolibrary.org/obo/IAO_0000027 -->

    <owl:Class rdf:about="http://purl.obolibrary.org/obo/IAO_0000027">
        <rdfs:label xml:lang="en">data item</rdfs:label>
        <rdfs:subClassOf rdf:resource="http://purl.obolibrary.org/obo/IAO_0000030"/>
        <obo:IAO_0000115 xml:lang="en">An information content entity that is intended to be a truthful statement about something (modulo, e.g., measurement precision or other systematic errors) and is constructed/acquired by a method which reliably tends to produce (approximately) truthful statements.</obo:IAO_0000115>
        <obo:IAO_0000118 xml:lang="en">data</obo:IAO_0000118>
        <obo:IAO_0000412 rdf:resource="http://purl.obolibrary.org/obo/obcs.owl"/>
    </owl:Class>
    


    <!-- http://purl.obolibrary.org/obo/IAO_0000030 -->

    <owl:Class rdf:about="http://purl.obolibrary.org/obo/IAO_0000030">
        <rdfs:label xml:lang="en">information content entity</rdfs:label>
        <rdfs:subClassOf rdf:resource="http://purl.obolibrary.org/obo/BFO_0000031"/>
        <obo:IAO_0000115 xml:lang="en">A generically dependent continuant that is about some thing.</obo:IAO_0000115>
        <obo:IAO_0000412 rdf:resource="http://purl.obolibrary.org/obo/obcs.owl"/>
    </owl:Class>
    


    <!-- http://purl.obolibrary.org/obo/OBCS_0000049 -->

    <owl:Class rdf:about="http://purl.obolibrary.org/obo/OBCS_0000049">
        <rdfs:label>accuracy</rdfs:label>
        <rdfs:subClassOf rdf:resource="http://purl.obolibrary.org/obo/OBCS_0000220"/>
        <obo:IAO_0000115>A data item that refers to the number of true positives and true negatives divided by the total number of observations.</obo:IAO_0000115>
        <obo:IAO_0000412 rdf:resource="http://purl.obolibrary.org/obo/obcs.owl"/>
    </owl:Class>
    


    <!-- http://purl.obolibrary.org/obo/OBCS_0000218 -->

    <owl:Class rdf:about="http://purl.obolibrary.org/obo/OBCS_0000218">
        <rdfs:label xml:lang="en">derived data from statistical analysis</rdfs:label>
        <rdfs:subClassOf rdf:resource="http://purl.obolibrary.org/obo/OBCS_0000233"/>
        <obo:IAO_0000118>statistic</obo:IAO_0000118>
        <obo:IAO_0000115>A data item that is derived from a statistical data analysis.</obo:IAO_0000115>
        <obo:IAO_0000412 rdf:resource="http://purl.obolibrary.org/obo/obcs.owl"/>
    </owl:Class>
    


    <!-- http://purl.obolibrary.org/obo/OBCS_0000220 -->

    <owl:Class rdf:about="http://purl.obolibrary.org/obo/OBCS_0000220">
        <rdfs:label xml:lang="en">derived data from inferential statistical analysis</rdfs:label>
        <rdfs:subClassOf rdf:resource="http://purl.obolibrary.org/obo/OBCS_0000218"/>
        <obo:IAO_0000115>A data item that is derived from an inferential statistical data analysis.</obo:IAO_0000115>
        <obo:IAO_0000118>inferential statistic</obo:IAO_0000118>
        <obo:IAO_0000412 rdf:resource="http://purl.obolibrary.org/obo/obcs.owl"/>
    </owl:Class>
    


    <!-- http://purl.obolibrary.org/obo/OBCS_0000233 -->

    <owl:Class rdf:about="http://purl.obolibrary.org/obo/OBCS_0000233">
        <rdfs:label xml:lang="en">transformed data item</rdfs:label>
        <rdfs:subClassOf rdf:resource="http://purl.obolibrary.org/obo/IAO_0000027"/>
        <obo:IAO_0000115>A data item that is produced as the output of a data transformation.</obo:IAO_0000115>
        <obo:IAO_0000412 rdf:resource="http://purl.obolibrary.org/obo/obcs.owl"/>
    </owl:Class>
</rdf:RDF>



<!-- Generated by the OWL API (version 3.2.4.1806) http://owlapi.sourceforge.net -->

