<?xml version="1.0"?>
<rdf:RDF xmlns="http://ontofox.hegroup.org/p63s94pd.owl#"
     xml:base="http://ontofox.hegroup.org/p63s94pd.owl"
     xmlns:data="http://www.ebi.ac.uk/swo/data/"
     xmlns:rdf="http://www.w3.org/1999/02/22-rdf-syntax-ns#"
     xmlns:owl="http://www.w3.org/2002/07/owl#"
     xmlns:xsd="http://www.w3.org/2001/XMLSchema#"
     xmlns:rdfs="http://www.w3.org/2000/01/rdf-schema#"
     xmlns:swo="http://www.ebi.ac.uk/swo/"
     xmlns:interface="http://www.ebi.ac.uk/swo/interface/"
     xmlns:obo="http://purl.obolibrary.org/obo/">
    <owl:Ontology rdf:about="http://ontofox.hegroup.org/p63s94pd.owl"/>
    


    <!-- 
    ///////////////////////////////////////////////////////////////////////////////////////
    //
    // Annotation properties
    //
    ///////////////////////////////////////////////////////////////////////////////////////
     -->

    <owl:AnnotationProperty rdf:about="http://www.w3.org/1999/02/22-rdf-syntax-ns#type"/>
    <owl:AnnotationProperty rdf:about="http://purl.obolibrary.org/obo/IAO_0000118">
        <rdfs:label xml:lang="en">alternative label</rdfs:label>
        <rdfs:label>alternative term</rdfs:label>
        <rdfs:label xml:lang="en">alternative term</rdfs:label>
        <obo:IAO_0000115 xml:lang="en">A label for a class or property that can be used to refer to the class or property instead of the preferred rdfs:label. Alternative labels should be used to indicate community- or context-specific labels, abbreviations, shorthand forms and the like.</obo:IAO_0000115>
        <obo:IAO_0000115 xml:lang="en">An alternative name for a class or property which means the same thing as the preferred name (semantically equivalent)</obo:IAO_0000115>
    </owl:AnnotationProperty>
    <owl:AnnotationProperty rdf:about="http://purl.obolibrary.org/obo/IAO_0000412">
        <rdfs:label xml:lang="en">imported from</rdfs:label>
    </owl:AnnotationProperty>
    <owl:AnnotationProperty rdf:about="http://purl.obolibrary.org/obo/IAO_0000115">
        <rdfs:label>textual definition</rdfs:label>
        <rdfs:label>definition</rdfs:label>
        <rdfs:label xml:lang="en">definition</rdfs:label>
        <obo:IAO_0000115 xml:lang="en">The official OBI definition, explaining the meaning of a class or property. Shall be Aristotelian, formalized and normalized. Can be augmented with colloquial definitions.</obo:IAO_0000115>
        <obo:IAO_0000115 xml:lang="en">The official definition, explaining the meaning of a class or property. Shall be Aristotelian, formalized and normalized. Can be augmented with colloquial definitions.</obo:IAO_0000115>
    </owl:AnnotationProperty>
    <owl:AnnotationProperty rdf:about="http://www.w3.org/2000/01/rdf-schema#label">
        <rdfs:label>label</rdfs:label>
    </owl:AnnotationProperty>
    


    <!-- 
    ///////////////////////////////////////////////////////////////////////////////////////
    //
    // Datatypes
    //
    ///////////////////////////////////////////////////////////////////////////////////////
     -->

    


    <!-- 
    ///////////////////////////////////////////////////////////////////////////////////////
    //
    // Classes
    //
    ///////////////////////////////////////////////////////////////////////////////////////
     -->

    


    <!-- http://purl.obolibrary.org/obo/BFO_0000015 -->

    <owl:Class rdf:about="http://purl.obolibrary.org/obo/BFO_0000015"/>
    


    <!-- http://purl.obolibrary.org/obo/BFO_0000023 -->

    <owl:Class rdf:about="http://purl.obolibrary.org/obo/BFO_0000023"/>
    


    <!-- http://purl.obolibrary.org/obo/BFO_0000031 -->

    <owl:Class rdf:about="http://purl.obolibrary.org/obo/BFO_0000031"/>
    


    <!-- http://purl.obolibrary.org/obo/IAO_0000030 -->

    <owl:Class rdf:about="http://purl.obolibrary.org/obo/IAO_0000030">
        <rdfs:label>information content entity</rdfs:label>
        <rdfs:label xml:lang="en">information content entity</rdfs:label>
        <rdfs:subClassOf rdf:resource="http://purl.obolibrary.org/obo/BFO_0000031"/>
        <obo:IAO_0000115>An information content entity is an entity that is generically dependent on some artifact and stands in relation of aboutness to some entity.</obo:IAO_0000115>
        <obo:IAO_0000115 xml:lang="en">A generically dependent continuant that is about some thing.</obo:IAO_0000115>
        <obo:IAO_0000412 rdf:resource="http://purl.obolibrary.org/obo/swo.owl"/>
    </owl:Class>
    


    <!-- http://www.ebi.ac.uk/swo/SWO_0000143 -->

    <owl:Class rdf:about="http://www.ebi.ac.uk/swo/SWO_0000143">
        <rdfs:label>data storage</rdfs:label>
        <rdfs:subClassOf rdf:resource="http://purl.obolibrary.org/obo/BFO_0000015"/>
        <obo:IAO_0000115>The storing of digital information. Often this is done for archiving and retrieval purposes.</obo:IAO_0000115>
        <obo:IAO_0000412 rdf:resource="http://purl.obolibrary.org/obo/swo.owl"/>
    </owl:Class>
    


    <!-- http://www.ebi.ac.uk/swo/data/SWO_3000053 -->

    <owl:Class rdf:about="http://www.ebi.ac.uk/swo/data/SWO_3000053">
        <rdfs:label xml:lang="en">Knowledge representation</rdfs:label>
        <rdfs:subClassOf rdf:resource="http://purl.obolibrary.org/obo/BFO_0000023"/>
        <obo:IAO_0000115>A knowledge representation role is a role borne by a data format which utilizes formalisms to make complex systems easier to design and build. Knowledge representation is the field of artificial intelligence devoted to representing information about the world in a form that a computer system can utilize to solve complex tasks.</obo:IAO_0000115>
        <obo:IAO_0000412 rdf:resource="http://purl.obolibrary.org/obo/swo.owl"/>
    </owl:Class>
    


    <!-- http://www.ebi.ac.uk/swo/interface/SWO_9000051 -->

    <owl:Class rdf:about="http://www.ebi.ac.uk/swo/interface/SWO_9000051">
        <rdfs:label>web service</rdfs:label>
        <rdfs:subClassOf rdf:resource="http://purl.obolibrary.org/obo/IAO_0000030"/>
        <obo:IAO_0000118>Web Service</obo:IAO_0000118>
        <obo:IAO_0000115>A web service is a software interface which works as a method of communication between two electronic devices over the World Wide Web and which is provided at a particular network address. There are two major classes of Web services: REST-compliant Web services, and arbitrary (or application-specific) Web services.</obo:IAO_0000115>
        <obo:IAO_0000412 rdf:resource="http://purl.obolibrary.org/obo/swo.owl"/>
    </owl:Class>
</rdf:RDF>



<!-- Generated by the OWL API (version 3.2.4.1806) http://owlapi.sourceforge.net -->

